proof/DDC/Language/SystemF2Data/Def.v
@@ -1,20 +1,78 @@
 
+Require Import DDC.Language.SystemF2.Ki.
+Require Import DDC.Language.SystemF2.KiJudge.
 Require Import DDC.Language.SystemF2.Ty.
 Require Import DDC.Base.
+Require Import Coq.Bool.Bool.
 
-
-(* Data Constructors *)
+(********************************************************************)
+(* Data Constructors
+   Carries a data constructor tag and an arity. *)
 Inductive datacon : Type :=
- | DataCon    : nat -> datacon.
+ | DataCon    : nat -> nat -> datacon.
 Hint Constructors datacon.
 
 
+Lemma beq_true_and_split
+ :  forall a1 a2
+ ,  true = a1 && a2
+ -> true = a1 /\ true = a2.
+Proof.
+ destruct a1; destruct a2; auto.
+Qed.
+
+
+Lemma beq_false_and_split
+ :  forall a1 a2
+ ,  false = a1 && a2
+ -> false = a1 \/ false = a2.
+Proof.
+ destruct a1; destruct a2; auto. 
+Qed.
+
+
+(* Boolean equality for data constructors. *)
+Lemma datacon_beq_eq
+ :  forall dc dc' 
+ ,  true = datacon_beq dc dc'
+ -> dc = dc'.
+Proof.
+ intros.
+ destruct dc.
+ destruct dc'.
+ simpl in H.
+  apply beq_true_and_split in H. inverts H.
+  apply beq_nat_eq in H0.
+  apply beq_nat_eq in H1.
+  burn.
+Qed.
+
+
+(* Boolean negation for data constructors. *)
+Lemma datacon_beq_false
+ :  forall dc 
+ ,  false = datacon_beq dc dc 
+ -> False.
+Proof.
+ intro.
+ destruct dc.
+ simpl.
+ intros.
+  apply beq_false_and_split in H.
+  inverts H.
+   induction n. false. auto.
+   induction n0. false. auto.
+Qed.
+
+
+(********************************************************************)
 (* Definitions. 
    Carries meta information about type and data constructors. *)
 Inductive def  : Type :=
  (* Definition of a data type constructor *)
  | DefDataType 
    :  tycon        (* Name of data type constructor *)
+   -> list ki      (* Kinds of type parameters *)
    -> list datacon (* Data constructors that belong to this type *)
    -> def
 
@@ -22,7 +80,7 @@ Inductive def  : Type :=
  | DefData 
    :  datacon      (* Name of data constructor *)
    -> list ty      (* Types of arguments *)
-   -> ty           (* Type  of constructed data *)
+   -> tycon        (* Type constructor of constructed data *)
    -> def.
 Hint Constructors def.
 
@@ -36,7 +94,7 @@ Definition defs  := list def.
    Returns None if it's not in the list. *)
 Fixpoint getTypeDef (tc: tycon) (ds: defs) : option def := 
  match ds with 
- | ds' :> DefDataType tc' _ as d
+ | ds' :> DefDataType tc' _ _ as d
  => if tycon_beq tc tc' 
      then  Some d
      else  getTypeDef tc ds'
@@ -60,33 +118,37 @@ Fixpoint getDataDef (dc: datacon) (ds: defs) : option def :=
  end.
 
 
-(* Boolean equality for data constructors. *)
-Lemma datacon_beq_eq
- :  forall dc dc' 
- ,  true = datacon_beq dc dc'
- -> dc = dc'.
-Proof.
- intros.
- destruct dc.
- destruct dc'.
- simpl in H.
- apply beq_nat_eq in H.
- auto.
-Qed.
+(********************************************************************)
+(* Check that a definition is ok. *)
+Inductive DEFOK : list def -> def -> Prop :=
+ (* Check that a data type definition is ok *)
+ | DefOkType
+   :  forall ds tc ks dcs
+      (* There must be at least one data constructor *)
+   ,  length dcs > 0
+      
+      (* All the data constructors must be present in the list of defs *)
+   -> Forall (fun dc => exists ddef, getDataDef dc ds = Some ddef) dcs
 
+   -> DEFOK ds (DefDataType tc ks dcs)
 
-(* Boolean negation for data constructors. *)
-Lemma datacon_beq_false
- :  forall dc 
- ,  false = datacon_beq dc dc 
- -> False.
-Proof.
- intro.
- destruct dc.
- simpl.
- intros.
-  induction n.
-  simpl in H. false.
-  simpl in H. auto.
-Qed.
+ (* Check that a data constructor definition is ok. *)
+ | DefOkData
+   :  forall tc ds ks dc dcs tsArgs
+      (* Get the data type def this data ctor belongs to *)
+   ,  getTypeDef tc ds = Some (DefDataType tc ks dcs)
+
+      (* Data ctor must be one of the ctors in the data type def *)
+   -> In dc dcs
+
+      (* All the ctor arg types must be well kinded in an environment
+         consistin of just the parameter types. *)
+   -> Forall (fun t => KIND ks t KStar) tsArgs
+
+   -> DEFOK ds (DefData dc tsArgs tc).
+
+(* Check that some data type definitions and their
+   associated constructors are ok *)
+Definition DEFSOK (ds: list def) : Prop :=
+  Forall (DEFOK ds) ds.
 
