proof/DDC/Language/SystemF2/KiJudge.v
@@ -70,25 +70,24 @@ Hint Resolve kind_empty_is_closed.
 Lemma kind_kienv_insert
  :  forall ke ix t k1 k2
  ,  KIND ke t k1
- -> KIND (insert ix k2 ke) (liftTT ix t) k1.
+ -> KIND (insert ix k2 ke) (liftTT 1 ix t) k1.
 Proof.
  intros. gen ix ke k1.
  induction t; intros; simpl; inverts_kind; eauto.
 
  Case "TVar".
-  lift_cases; intros; auto.
+  lift_cases; intros; nnat; auto.
 
  Case "TForall".
   apply KIForall.
-  rewrite insert_rewind.
-  apply IHt. auto.
+  rewrite insert_rewind. auto.
 Qed.
 
 
 Lemma kind_kienv_weaken
  :  forall ke t k1 k2
- ,  KIND  ke         t           k1
- -> KIND (ke :> k2) (liftTT 0 t) k1.
+ ,  KIND  ke         t             k1
+ -> KIND (ke :> k2) (liftTT 1 0 t) k1.
 Proof.
  intros.
  assert (ke :> k2 = insert 0 k2 ke). simpl.
