proof/DDC/Language/SystemF2/TyBase.v
@@ -1,0 +1,54 @@
+
+Require Export DDC.Language.SystemF2.Ki.
+
+(* Type Constructors. *)
+Inductive tycon : Type :=
+ | TyConFun  : tycon
+ | TyConData : nat   -> ki -> tycon.
+Hint Constructors tycon.
+
+(* Type Expressions. *)
+Inductive ty  : Type :=
+ | TCon      : tycon -> ty
+ | TVar      : nat   -> ty
+ | TForall   : ty    -> ty
+ | TApp      : ty    -> ty -> ty.
+Hint Constructors ty.
+
+
+(* Baked in types. *)
+Definition tFun (t1: ty) (t2: ty)
+ := TApp (TApp (TCon TyConFun) t1) t2.
+Hint Unfold tFun.
+
+
+(* Get the type constructor of a type, if any *)
+Fixpoint getCtorOfType (tt: ty) : option tycon :=
+ match tt with
+ | TCon tc   => Some tc
+ | TApp t1 _ => getCtorOfType t1
+ | _         => None
+ end.
+
+
+(* Construct a type application from a constructor type
+   and a list of argument types. *)
+Fixpoint makeTApps (t1: ty) (tt: list ty) : ty :=
+ match tt with
+ | nil     => t1
+ | t :: ts => makeTApps (TApp t1 t) ts
+ end.
+
+
+
+(* Break apart a type application into the constructor type
+   and a list of argument types. *)
+Fixpoint takeTApps (tt: ty) : (ty * list ty) :=
+ match tt with
+ | TApp t1 t2 => match takeTApps t1 with
+                 | (t11, t1s) => (t1, snoc t2 t1s )
+                 end
+ | _          => (tt, nil)
+ end.
+
+
