proof/DDC/Language/SystemF2/TyLift.v
@@ -1,0 +1,50 @@
+
+Require Export DDC.Language.SystemF2.TyBase.
+
+
+(*******************************************************************)
+(* Lift type indices that are at least a certain depth. *)
+Fixpoint liftTT (n: nat) (d: nat) (tt: ty) : ty :=
+  match tt with
+  |  TVar ix
+  => if le_gt_dec d ix
+      then TVar (ix + n)
+      else tt
+
+  |  TCon _     => tt
+
+  |  TForall t 
+  => TForall (liftTT n (S d) t)
+
+  |  TApp t1 t2
+  => TApp    (liftTT n d t1) (liftTT n d t2)
+  end.
+Hint Unfold liftTT.
+
+
+(* Tactic to help deal with lifting functions *)
+Ltac lift_cases 
+ := match goal with 
+     |  [ |- context [le_gt_dec ?n ?n'] ]
+     => case (le_gt_dec n n')
+    end.
+
+
+(********************************************************************)
+(* Changing the order of lifting. *)
+Lemma liftTT_liftTT
+ :  forall d d' t
+ ,  liftTT 1 d              (liftTT 1 (d + d') t) 
+ =  liftTT 1 (1 + (d + d')) (liftTT 1 d t).
+Proof.
+ intros. gen d d'.
+ induction t; intros; simpl; try burn.
+
+ Case "TVar".
+  repeat (unfold liftTT; lift_cases; intros); burn.
+
+ Case "TForall".
+  assert (S (d + d') = (S d) + d'). omega. rewrite H. 
+  rewrite IHt. auto.
+Qed.  
+
