proof/DDC/Language/SystemF2/TySubst.v
@@ -1,0 +1,128 @@
+
+Require Export DDC.Language.SystemF2.TyBase.
+Require Export DDC.Language.SystemF2.TyLift.
+
+
+(********************************************************************)
+(* Substitution of Types in Types. *)
+Fixpoint substTT (d: nat) (u: ty) (tt: ty) : ty 
+ := match tt with
+    | TVar ix
+    => match nat_compare ix d with
+       | Eq => u
+       | Gt => TVar (ix - 1)
+       | _  => TVar  ix
+       end
+
+    |  TCon _     
+    => tt
+ 
+    |  TForall t  
+    => TForall (substTT (S d) (liftTT 1 0 u) t)
+
+    |  TApp t1 t2 
+    => TApp (substTT d u t1) (substTT d u t2)
+  end.
+
+
+Fixpoint substTTs (d: nat) (us: list ty) (tt: ty) :=
+ match us with
+ | nil      => tt
+ | u :: us' => substTTs d us' 
+                 (substTT d (liftTT (List.length us') 0 u)
+                            tt)
+ end.
+
+
+(********************************************************************)
+(* If we lift at depth d, this creates an empty space and
+   substituting into it doens't do anything. *)
+Lemma substTT_liftTT
+ :  forall d t1 t2
+ ,  substTT d t2 (liftTT 1 d t1) = t1.
+Proof.
+ intros. gen d t2.
+ induction t1; intros; simpl; try burn.
+
+ Case "TVar".
+  lift_cases; unfold substTT;
+   fbreak_nat_compare; intros;
+   burn.
+Qed.
+
+
+(* Lifting after substitution *)
+Lemma liftTT_substTT
+ :  forall n n' t1 t2
+ ,  liftTT 1 n (substTT (n + n') t2 t1)
+ =  substTT (1 + n + n') (liftTT 1 n t2) (liftTT 1 n t1).
+Proof.
+ intros. gen n n' t2.
+ induction t1; intros; simpl; try burn.
+
+ Case "TVar".
+  repeat (simpl; fbreak_nat_compare; 
+          try lift_cases; try intros);
+   burn.
+
+ Case "TForall".
+  simpl.
+  rewrite (IHt1 (S n) n'). simpl.
+  rewrite (liftTT_liftTT 0 n). auto.
+
+ Case "TApp".
+  rewrite IHt1_1. 
+  rewrite IHt1_2. auto.
+Qed.
+
+
+Lemma liftTT_substTT'
+ :  forall n n' t1 t2
+ ,  liftTT 1 (n + n') (substTT n t2 t1)
+ =  substTT n (liftTT 1 (n + n') t2) (liftTT 1 (1 + n + n') t1).
+Proof.
+ intros. gen n n' t2.
+ induction t1; intros; eauto.
+
+ Case "TVar".
+  repeat ( unfold liftTT; unfold substTT; fold liftTT; fold substTT
+         ; try lift_cases; try fbreak_nat_compare
+         ; intros); try burn.
+
+ Case "TForall".
+  simpl. f_equal.
+  rewrite (IHt1 (S n) n'). f_equal.
+   simpl. rewrite (liftTT_liftTT 0 (n + n')). auto.
+
+ Case "TApp".
+  simpl. f_equal.
+   apply IHt1_1.
+   apply IHt1_2.
+Qed.
+
+
+(* Commuting substitutions. *)
+Lemma substTT_substTT
+ :  forall n m t1 t2 t3
+ ,  substTT (n + m) t3 (substTT n t2 t1)
+ =  substTT n (substTT (n + m) t3 t2)
+              (substTT (1 + n + m) (liftTT 1 n t3) t1).
+Proof.
+ intros. gen n m t2 t3.
+ induction t1; intros; auto.
+
+ Case "TVar".
+  repeat (simpl; fbreak_nat_compare); try burn.
+  rewrite substTT_liftTT. auto.
+
+ Case "TForall".
+  simpl. f_equal.
+  rewrite (IHt1 (S n) m). f_equal.
+   simpl. rewrite (liftTT_substTT 0 (n + m)). auto.
+   simpl. rewrite (liftTT_liftTT 0 n). auto.  
+
+ Case "TApp".
+  simpl. f_equal.
+   apply IHt1_1.
+   apply IHt1_2.
+Qed.
